06: add local lemma proof for beta reduction

tapl/tapl/s06nameless.lean
@@ -187,13 +187,30 @@ theorem cbv_implies_cbn (h : CBValueNormalizable t) : CBNameNormalizable t := by
     · contradiction
     · sorry
 
-def beta_red (k : ℕ) (t s : BLTerm) := shift_down_from k (subst k (shift_up_from k s) t)
+def shift_up_from_iter (k : Nat) (s : BLTerm) :=
+  match k with
+  | 0 => shift_up s
+  | k_1 + 1 => shift_up (shift_up_from_iter k_1 s)
 
-inductive Step : BLTerm → BLTerm → Prop
-| refl : Step t t
-| abs : Step t t' → Step (.Abs t) (.Abs t')
-| app : Step t t' → Step s s' → Step (.App t s) (.App t' s')
-| beta : Step t t' → Step s s' → Step (.App (.Abs t) s) (beta_red 0 t' s')
+
+def shift_up_iter (k : Nat) (s : BLTerm) :=
+  match k with
+  | 0 => s
+  | k_1 + 1 => shift_up (shift_up_iter k_1 s)
+
+def shift_down_from_iter (k : Nat) (n : Nat) (s : BLTerm) :=
+  match k with
+  | 0 => shift_down_from n s
+  | k_1 + 1 => shift_down (shift_down_from_iter k_1 n s)
+
+def betar (k : Nat) (t s : BLTerm) : BLTerm :=
+  match t with
+  | .Var x => if x = k then s else if x < k then .Var x else .Var x.pred
+  | .Abs t1 => (betar (k + 1) t1 (shift_up s)).Abs
+  | .App t1 t2 => (betar k t1 s).App (betar k t2 s)
+
+def beta_red (k : ℕ) (t s : BLTerm) :=
+  shift_down_from k (substN k (shift_up_from k s) t)
 
 theorem shift_up_down (t : BLTerm) :
   shift_down_from x (shift_up_from x t) = t := by
@@ -211,145 +228,321 @@ theorem shift_up_down (t : BLTerm) :
 
 lemma beta_dist (t1 t2 s : BLTerm) :
   beta_red k (t1.App t2) s = (beta_red k t1 s).App (beta_red k t2 s) := by
-    rw [beta_red, beta_red, subst, shift_down_from]
+    rw [beta_red, beta_red, substN, shift_down_from]
     rfl
 
---probably correct and needs a generalization
-lemma beta_some_lemma (t s : BLTerm) :
-  n = 0 → (beta_red n (shift_up_from (k + 1) t) (shift_up_from k s)) =
-  shift_up_from k (beta_red n t s) := by
-    unhygienic induction t generalizing n k
-    { repeat rw [beta_red]
-      grind [Nat.pred_eq_sub_one, shift_down_from, shift_up_from, shift_up_down, subst] }
-    { simp [beta_red, subst, shift_down_from, shift_up_from]
-      intro heq
-      have := t_ih (n := n + 1) (k := k + 1) sorry
-      simp [beta_red] at this
-      sorry }
-    rw [beta_dist, shift_up_from, shift_up_from, beta_dist]
+lemma shift_comp_one :
+  shift_up_from d (shift_up_from (k + d) t) = shift_up_from (k + d + 1) (shift_up_from d t) := by
+  unhygienic induction t generalizing d <;> grind [shift_up, shift_up_from]
+
+lemma beta_eq (t s : BLTerm) :
+  beta_red k t s = betar k t s := by
+    unhygienic induction t generalizing s k
+    { rw [beta_red, betar, substN]
+      grind [shift_up_from, substN, shift_down_from, Nat.pred_eq_sub_one, shift_up_down] }
+    { rw [beta_red, substN]
+      rw [betar, shift_down_from]
+      have eq_lemma := shift_comp_one (d := 0) (t := s) (k := k)
+      grind [shift_up, beta_red] }
+    rw [beta_dist, betar]
     grind
 
-lemma beta_shift (t t' : BLTerm) :
-  Step t t' → Step (shift_up_from k t) (shift_up_from k t') := by
-    intro ht
-    unhygienic induction ht generalizing k
-    { apply Step.refl }
-    { repeat rw [shift_up_from]
-      apply Step.abs
-      grind }
-    { repeat rw [shift_up_from]
-      apply Step.app <;> grind }
-    repeat rw [shift_up_from]
-    have h1 := a_ih (k := k + 1)
-    have h2 := a_ih_1 (k := k)
-    have := Step.beta h1 h2
-    rw [beta_some_lemma] at this
-    { apply this }
-    omega
 
--- should be correct
-theorem step_beta (s t s' t' : BLTerm) :
-  Step s s' → Step t t' → Step (beta_red 0 t s) (beta_red 0 t' s') := by
-    intro hs ht
-    unhygienic induction t generalizing t' s s'
-    { cases ht
-      rw [beta_red, subst, beta_red, subst]
-      split_ifs with h
-      { rw [shift_up_down, shift_up_down]
-        exact hs }
-      apply Step.refl }
-    { --simp only [beta_red, subst, zero_add, shift_down_from]
-      unhygienic cases ht
-      { apply Step.abs
-        sorry }
-      apply Step.abs
-      sorry }
-    unhygienic cases ht
-    { rw [beta_dist, beta_dist]
-      apply Step.app
-      { apply t1_ih s s' t1 hs (by grind [Step]) }
-      apply t2_ih s s' t2 hs (by grind [Step]) }
-    { rw [beta_dist, beta_dist]
-      apply Step.app
-      { apply t1_ih s s' t'_1 hs a }
-      apply t2_ih s s' s'_1 hs a_1 }
-    rw [beta_dist]
-    sorry
+inductive SStep : BLTerm → BLTerm → Prop
+| abs : SStep t t' → SStep (.Abs t) (.Abs t')
+| appl : SStep t t' → SStep (.App t s) (.App t' s)
+| appr : SStep s s' → SStep (.App t s) (.App t s')
+| beta : SStep (.App (.Abs t) s) (betar 0 t s)
 
-theorem step_inj (s t1 t2 : BLTerm) :
-  Step s t1 → Step s t2 → ∃ r, Step t1 r ∧ Step t2 r := by
-    unhygienic induction s generalizing t1 t2
-    { grind [Step] }
-    { intro h1 h2
-      unhygienic cases h1
-      { exists t2
-        grind [Step] }
-      unhygienic cases h2
-      { exists t'.Abs
-        grind [Step] }
-      rcases t_ih t' t'_1 a a_1 with ⟨r, hr⟩
-      exists .Abs r
-      grind [Step] }
+inductive MultiSStep : BLTerm → BLTerm → Prop
+| refl : MultiSStep s s
+| step : MultiSStep s1 s2 → SStep s s1 → MultiSStep s s2
+
+lemma ms_trans :
+  MultiSStep t t1 → MultiSStep t1 t2 → MultiSStep t t2 := by
     intro h1 h2
-    unhygienic cases h1 <;> unhygienic cases h2
-    { exists t1.App t2
-      grind [Step] }
+    unhygienic induction h1
+    { exact h2 }
+    apply MultiSStep.step
+    { apply a_ih h2 }
+    exact a_1
+
+lemma ms_app :
+  MultiSStep t t' → MultiSStep s s' → MultiSStep (t.App s) (t'.App s') := by
+    intro ht hs
+    apply ms_trans (t1 := t'.App s)
+    { unhygienic induction ht
+      { apply MultiSStep.refl }
+      apply MultiSStep.step
+      { apply a_ih }
+      grind [SStep] }
+    unhygienic induction hs
+    { apply MultiSStep.refl }
+    apply MultiSStep.step
+    { apply a_ih }
+    grind [SStep]
+
+lemma ms_abs :
+  MultiSStep t t' → MultiSStep t.Abs t'.Abs := by
+    intro ht
+    unhygienic induction ht
+    { apply MultiSStep.refl }
+    apply MultiSStep.step
+    { apply a_ih }
+    grind [SStep]
+
+lemma shift_comp :
+  shift_up_iter d (shift_up_from k s) = shift_up_from (k + d) (shift_up_iter d s) := by
+  unhygienic induction d generalizing k s
+  { grind [shift_up_iter] }
+  repeat rw [shift_up_iter]
+  rw [a, shift_up, shift_up]
+  have := shift_comp_one (d := 0) (k := k + n) (t := (shift_up_iter n s))
+  grind
+
+lemma beta_shift_lemma_gen (t s : BLTerm) (d : Nat) :
+  (betar d (shift_up_from (k + 1 + d) t) (shift_up_iter d (shift_up_from k s))) =
+  shift_up_from (k + d) (betar d t (shift_up_iter d s)) := by
+    unhygienic induction t generalizing d
+    { rw [shift_up_from]
+      split_ifs
+      { rw [betar, betar]
+        split_ifs
+        { apply shift_comp }
+        { rw [shift_up_from]
+          grind }
+        grind [shift_up_from, Nat.pred_eq_sub_one] }
+      rw [betar, betar]
+      split_ifs <;> try grind [shift_up_from, Nat.pred_eq_sub_one] }
+    { rw [shift_up_from, betar, betar, shift_up_from]
+      have ih := t_ih (d := d + 1)
+      rw [shift_up_iter, shift_up_iter] at ih
+      grind }
+    rw [betar, shift_up_from, betar, shift_up_from]
+    grind
+
+lemma shift_up_step (s s' : BLTerm) :
+  SStep s s' → SStep (shift_up_from k s) (shift_up_from k s') := by
+    intro hs
+    unhygienic induction hs generalizing k
+    { repeat rw [shift_up_from]
+      grind [SStep] }
+    { rw [shift_up_from, shift_up_from]
+      grind [SStep] }
+    { rw [shift_up_from, shift_up_from]
+      grind [SStep] }
+    repeat rw [shift_up_from]
+    have := SStep.beta (t := (shift_up_from (k + 1) t)) (s := (shift_up_from k s_1))
+    have eq := beta_shift_lemma_gen t s_1 0 (k := k)
+    simp only [add_zero, shift_up_iter] at eq
+    rw [eq] at this
+    exact this
+
+lemma shift_beta_one (d k : Nat) (s_1 s : BLTerm) :
+  shift_up_from d (betar (k + d) s_1 (shift_up_iter d s)) =
+  betar (k + d + 1) (shift_up_from d s_1) (shift_up_iter d (shift_up_from 0 s)) := by
+  unhygienic induction s_1 generalizing d
+  { rw [betar, shift_up_from]
+    split_ifs <;> try grind [betar, shift_up_iter, Nat.pred_eq_sub_one, shift_up_from]
+    rw [betar]
+    split_ifs <;> try omega
+    simp [shift_comp] }
+  { simp only [betar, shift_up_from]
+    have ih := t_ih (d := d + 1)
+    grind [shift_up_iter] }
+  grind [betar, shift_up_from]
+
+lemma shift_iter_beta :
+  shift_up_iter d (betar k s_1 s) =
+  betar (k + d) (shift_up_iter d s_1) (shift_up_iter d s) := by
+  unhygienic induction d
+  { grind [shift_up_iter] }
+  repeat rw [shift_up_iter]
+  rw [a]
+  have := shift_beta_one 0 (k + n) (shift_up_iter n s_1) (shift_up_iter n s)
+  repeat rw [shift_up]
+  repeat rw [shift_up_iter] at this
+  grind
+
+def shift_iter_dir (k d : Nat) : BLTerm → BLTerm
+| .Var x => if x < k then .Var x else .Var (x + d)
+| .Abs t => (shift_iter_dir (k + 1) d t).Abs
+| .App t1 t2 => (shift_iter_dir k d t1).App (shift_iter_dir k d t2)
+
+lemma inner_shift_iter (d : Nat) (t : BLTerm) :
+  shift_up_iter (d + 1) t = shift_up_iter d (shift_up t) := by
+    induction d <;> grind [shift_up_iter]
+
+lemma shift_iter_eq (d : Nat) (t : BLTerm) :
+  shift_iter_dir 0 d t = shift_up_iter d t := by
+    unhygienic induction d generalizing t
+    { rw [shift_up_iter]
+      have zero_lem :
+        ∀ k,
+        shift_iter_dir k 0 t = t := by
+          induction t <;> grind [shift_iter_dir]
+      rw [zero_lem] }
+    rw [inner_shift_iter]
+    rw [←a]
+    rw [shift_up]
+    have zero_stat:
+      ∀ k,
+        shift_iter_dir k (n + 1) t = shift_iter_dir k n (shift_up_from k t) := by
+        unhygienic induction t <;> grind [shift_iter_dir, shift_up_from]
+    rw [zero_stat]
+
+lemma beta_shift_iter (d : Nat) :
+  betar d (shift_up_iter (d + 1) t) s = shift_up_iter d t := by
+    repeat rw [←shift_iter_eq]
+    have gen_lemma :
+      ∀ k,
+      betar (d + k) (shift_iter_dir k (d + 1) t) s = shift_iter_dir k d t := by
+        intro k
+        unhygienic induction t generalizing k s
+        { grind [shift_iter_dir, betar, Nat.pred_eq_sub_one] }
+        { repeat rw [shift_iter_dir]
+          rw [betar]
+          have := t_ih (s := shift_up s)
+          grind }
+        grind [betar, shift_iter_dir]
+    grind
+
+lemma beta_beta (d : Nat) (t_1 s s_1 : BLTerm) :
+  (betar d
+    (betar (k + d + 1) t_1 (shift_up (shift_up_iter d s)))
+    (shift_up_iter d (betar k s_1 s))) =
+  (betar (k + d) (betar d t_1 (shift_up_iter d s_1)) (shift_up_iter d s)) := by
+    unhygienic induction t_1 generalizing d
+    { repeat rw [betar]
+      split_ifs <;> try grind [Nat.pred_eq_sub_one, betar]
+      { rw [betar]
+        split_ifs <;> try grind [Nat.pred_eq_sub_one]
+        have := beta_shift_iter d (t := s) (s := (shift_up_iter d (betar k s_1 s)))
+        rw [shift_up_iter] at this
+        rw [this] }
+      rw [betar, if_pos]
+      { rw [shift_iter_beta] }
+      omega }
+    { repeat rw [betar]
+      have ih := t_ih (d := d + 1)
+      grind [shift_up_iter] }
+    repeat rw [betar]
+    grind
+
+lemma beta_step_l (k : Nat) (t t' s : BLTerm) :
+  SStep t t' → SStep (betar k t s) (betar k t' s) := by
+    intro ht
+    unhygienic induction ht generalizing s k
+    { rw [betar, betar]
+      grind [SStep] }
+    { rw [betar, betar]
+      grind [SStep] }
+    { rw [betar, betar]
+      grind [SStep] }
+    rw [betar, betar]
+    rename_i s_1
+    have := SStep.beta (t := (betar (k + 1) t_1 (shift_up s))) (s := (betar k s_1 s))
+    have lemma_2 := beta_beta 0 t_1 s s_1 (k := k)
+    simp only [add_zero, shift_up_iter] at lemma_2
+    grind
+
+lemma beta_step_r (t s s' : BLTerm) (k : Nat) :
+  MultiSStep s s' → MultiSStep (betar k t s) (betar k t s') := by
+    intro ht
+    unhygienic induction t generalizing s s' k
+    { rw [betar, betar]
+      split_ifs
+      { apply ht }
+      { apply MultiSStep.refl }
+      apply MultiSStep.refl }
+    { rw [betar, betar]
+      apply ms_abs
+      apply t_ih (shift_up s) (shift_up s') _
+      rw [shift_up, shift_up]
+      unhygienic induction ht
+      { apply MultiSStep.refl }
+      apply MultiSStep.step
+      { apply a_ih }
+      apply shift_up_step
+      apply a_1 }
+    rw [betar, betar]
+    apply ms_app <;> grind
+
+theorem step_diamond (s t1 t2 : BLTerm) :
+  SStep s t1 → SStep s t2 → ∃ r, MultiSStep t1 r ∧ MultiSStep t2 r := by
+    intro h1 h2
+    unhygienic induction h1 generalizing t2 <;> unhygienic cases h2
+    { rcases a_ih t'_1 a_1 with ⟨r, hr⟩
+      exists r.Abs
+      grind [ms_abs] }
+    { rcases a_ih t'_1 a_1 with ⟨r, hr⟩
+      exists r.App s_1
+      grind [ms_app, MultiSStep] }
     { exists t'.App s'
-      grind [Step] }
-    { exists beta_red 0 t' s'
-      grind [Step] }
-    { exists t'.App s'
-      grind [Step] }
-    { rcases t1_ih t' t'_1 a a_2 with ⟨t2, ht2⟩
-      rcases t2_ih s' s'_1 a_1 a_3 with ⟨s2, hs2⟩
-      exists t2.App s2
-      grind [Step] }
-    { rcases t2_ih s' s'_1 a_1 a_3 with ⟨s2, hs2⟩
-      unhygienic cases a
-      { exists beta_red 0 t'_1 s2
-        constructor
-        { apply Step.beta a_2 hs2.1 }
-        apply step_beta _ _ _ _ hs2.2
-        apply Step.refl }
-      rcases t1_ih t'_1.Abs t'_2.Abs (by grind [Step]) (by grind [Step]) with ⟨t2, ht2⟩
-      unhygienic cases t2
-      { grind [Step] }
-      { exists beta_red 0 t_1 s2
-        constructor
-        { apply Step.beta (by grind [Step]) hs2.1 }
-        apply step_beta _ _ _ _ hs2.2
-        grind [Step] }
-      grind [Step] }
-    { exists beta_red 0 t' s'
-      grind [Step] }
-    { rcases t2_ih s' s'_1 a_1 a_3 with ⟨s2, hs2⟩
-      unhygienic cases a_2
-      { exists beta_red 0 t' s2
-        constructor
-        { apply step_beta _ _ _ _ hs2.1
-          apply Step.refl    }
-        apply Step.beta a hs2.2 }
-      rcases t1_ih t'.Abs t'_2.Abs (by grind [Step]) (by grind [Step]) with ⟨t2, ht2⟩
-      unhygienic cases t2
-      { grind [Step] }
-      { exists beta_red 0 t_1 s2
-        constructor
-        { apply step_beta _ _ _ _ hs2.1
-          grind [Step] }
-        apply Step.beta (by grind [Step]) hs2.2 }
-      grind [Step] }
-    rcases t1_ih t'.Abs t'_1.Abs (by grind [Step]) (by grind [Step]) with ⟨r1, hr1⟩
-    rcases t2_ih _ _ a_1 a_3 with ⟨r2, hr2⟩
-    unhygienic cases r1
-    { grind [Step] }
-    { exists beta_red 0 t_1 r2
+      grind [ms_app, MultiSStep] }
+    { unhygienic cases a
+      exists betar 0 t'_1 s_1
       constructor
-      { apply step_beta _ _ _ _ hr2.1
-        grind [Step] }
-      apply step_beta _ _ _ _ hr2.2
-      grind [Step] }
-    grind [Step]
+      { apply MultiSStep.step
+        { apply MultiSStep.refl }
+        apply SStep.beta }
+      apply MultiSStep.step
+      { apply MultiSStep.refl }
+      apply beta_step_l _ _ _ _ a_1 }
+    { exists t'.App s'
+      grind [MultiSStep, ms_app] }
+    { rcases a_ih s'_1 a_1 with ⟨r, hr⟩
+      exists t.App r
+      grind [MultiSStep, ms_app] }
+    { exists betar 0 t_1 s'
+      constructor
+      { apply MultiSStep.step
+        { apply MultiSStep.refl }
+        apply SStep.beta }
+      have := MultiSStep.step (MultiSStep.refl) a
+      apply beta_step_r _ _ _ _ this }
+    { unhygienic cases a
+      exists betar 0 t'_1 s_1
+      constructor
+      { apply MultiSStep.step
+        { apply MultiSStep.refl }
+        apply beta_step_l _ _ _ _ a_1 }
+      apply MultiSStep.step
+      { apply MultiSStep.refl }
+      apply SStep.beta }
+    { exists betar 0 t s'
+      constructor
+      { have := MultiSStep.step (MultiSStep.refl) a
+        apply beta_step_r _ _ _ _ this }
+      apply MultiSStep.step
+      { apply MultiSStep.refl }
+      apply SStep.beta }
+    exists betar 0 t s_1
+    grind [MultiSStep.refl]
 
-end Semantics
+theorem multistep_diamond (s t1 t2 : BLTerm) :
+  MultiSStep s t1 → MultiSStep s t2 → ∃ r, MultiSStep t1 r ∧ MultiSStep t2 r := by
+    intro h1 h2
+    unhygienic induction h1 generalizing t2
+    { exists t2
+      grind [MultiSStep] }
+    unhygienic induction h2 generalizing s2 s1
+    { exists s2
+      grind [MultiSStep] }
+    rename_i s3 s4 hms hs ih
+    rcases step_diamond s_2 _ _ hs a_1 with ⟨r, hr1, hr2⟩
+    rcases a_ih _ hr2 with ⟨r1, hr3⟩
+    have : MultiSStep s3 r1 := by
+      apply ms_trans
+      { apply hr1 }
+      apply hr3.2
+    unhygienic cases this
+    { exists s4
+      grind [ms_trans, MultiSStep] }
 
-end Nameless
+    rcases ih (s2 := r1) (s1 := s1_1) a_2 a_3
+      (by
+        intro t3 ht3
+        sorry) with ⟨ans, hans⟩
+    exists ans
+    grind [ms_trans]
